some clean and an example using function pointer

compiler_test/c_progs/func_app_ptr.c
@@ -1,0 +1,13 @@
+#include <stdio.h>
+
+// Define a function
+int add(int x, int y) {
+    return x + y;
+}
+
+int main() {
+    int (*x)(int, int) = add;
+    int r = x(3,4);
+    return r;
+}
+
