compiler_test/cond3.c
@@ -1,5 +1,0 @@
-#include<stdio.h>
-int main() {
-	if (1) { return 1; }
-        else return 0;
-}
