compiler_test/cond4.c
@@ -1,7 +1,0 @@
-#include <stdio.h>
-int main() {
-	if (1 < 2) {
-		int r = 2 * 2;
-                return r; }
-        else return 0;
-}
