compiler_test/beepl_test/BeePL_progs.v
@@ -1,9 +1,9 @@
-
 Require Import AST Maps Ctypes.
-Require Import BeePL BeeTypes Errors BeePL_typechecker Csyntaxdefs BeePL_Option_Struct. 
+Require Import BeePL BeeTypes Errors BeePL_typechecker Csyntaxdefs. 
 From Coq Require Import String.
 
-Require Import BeePL_add. (* BeePL_cond BeePL_app BeePL_div_zero BeePL_div_zero1 BeePL_external_call BeePL_ref.
+Require Import BeePL_add BeePL_add_ptr. 
+(* BeePL_cond BeePL_app BeePL_div_zero BeePL_div_zero1 BeePL_external_call BeePL_ref.
 Require Import BeePL_struct_ex2 BeePL_for_ex1 BeePL_for_ex2 BeePL_globvar1.
 Require Import BeePL_bpf_get_prandom BeePL_bpf_ktime_get_ns.*) (*BeePL_null_ptr BeePL_match_fail_ex1.*)
 
@@ -33,11 +33,11 @@ Proof.
   unfold build_bcomposite_env; simpl; reflexivity.
 Qed.
 
-Definition example1 : BeePL.program := @mkbprogram BeePL_add.bcomposites 
-                                                   BeePL_add.global_definitions 
-                                                   BeePL_add.public_idents 
-                                                   BeePL_add._main 
-                                                   BeePL_add.bcomposite_correct
-                                                   BeePL_add.ident_to_string.
+Definition example1 : BeePL.program := @mkbprogram BeePL_add_ptr.bcomposites 
+                                                   BeePL_add_ptr.global_definitions 
+                                                   BeePL_add_ptr.public_idents 
+                                                   BeePL_add_ptr._main 
+                                                   BeePL_add_ptr.bcomposite_correct
+                                                   BeePL_add_ptr.ident_to_string.
 
 
