compiler_test/c_progs/func_app.v
@@ -15,7 +15,7 @@ Module Info.
   Definition abi := "apple".
   Definition bitsize := 64.
   Definition big_endian := false.
-  Definition source_file := "compiler_test/globvar1.c".
+  Definition source_file := "compiler_test/c_progs/func_app.c".
 End Info.
 
 Definition ___builtin_annot : ident := $"__builtin_annot".
@@ -73,69 +73,63 @@ Definition ___compcert_va_float64 : ident := $"__compcert_va_float64".
 Definition ___compcert_va_int32 : ident := $"__compcert_va_int32".
 Definition ___compcert_va_int64 : ident := $"__compcert_va_int64".
 Definition ___stringlit_1 : ident := $"__stringlit_1".
-Definition _a : ident := $"a".
 Definition _add : ident := $"add".
-Definition _b : ident := $"b".
 Definition _main : ident := $"main".
 Definition _printf : ident := $"printf".
+Definition _result : ident := $"result".
+Definition _x : ident := $"x".
+Definition _y : ident := $"y".
 
 Definition v___stringlit_1 := {|
-  gvar_info := (tarray tschar 3);
-  gvar_init := (Init_int8 (Int.repr 37) :: Init_int8 (Int.repr 100) ::
-                Init_int8 (Int.repr 0) :: nil);
+  gvar_info := (tarray tschar 12);
+  gvar_init := (Init_int8 (Int.repr 82) :: Init_int8 (Int.repr 101) ::
+                Init_int8 (Int.repr 115) :: Init_int8 (Int.repr 117) ::
+                Init_int8 (Int.repr 108) :: Init_int8 (Int.repr 116) ::
+                Init_int8 (Int.repr 58) :: Init_int8 (Int.repr 32) ::
+                Init_int8 (Int.repr 37) :: Init_int8 (Int.repr 100) ::
+                Init_int8 (Int.repr 10) :: Init_int8 (Int.repr 0) :: nil);
   gvar_readonly := true;
   gvar_volatile := false
 |}.
 
-Definition v_a := {|
-  gvar_info := tint;
-  gvar_init := (Init_space 4 :: nil);
-  gvar_readonly := false;
-  gvar_volatile := false
-|}.
-
-Definition v_b := {|
-  gvar_info := tint;
-  gvar_init := (Init_space 4 :: nil);
-  gvar_readonly := false;
-  gvar_volatile := false
-|}.
-
 Definition f_add := {|
-  fn_return := tvoid;
+  fn_return := tint;
   fn_callconv := cc_default;
-  fn_params := nil;
+  fn_params := ((_x, tint) :: (_y, tint) :: nil);
   fn_vars := nil;
   fn_body :=
-(Sdo (Ecall
-       (Evalof
-         (Evar _printf (Tfunction (Tcons (tptr tschar) Tnil) tint
-                         {|cc_vararg:=(Some 1); cc_unproto:=false; cc_structret:=false|}))
-         (Tfunction (Tcons (tptr tschar) Tnil) tint
-           {|cc_vararg:=(Some 1); cc_unproto:=false; cc_structret:=false|}))
-       (Econs
-         (Evalof (Evar ___stringlit_1 (tarray tschar 3)) (tarray tschar 3))
-         (Econs
-           (Ebinop Oadd (Evalof (Evar _a tint) tint)
-             (Evalof (Evar _b tint) tint) tint) Enil)) tint))
+(Sreturn (Some (Ebinop Oadd (Evalof (Evar _x tint) tint)
+                 (Evalof (Evar _y tint) tint) tint)))
 |}.
 
 Definition f_main := {|
   fn_return := tint;
   fn_callconv := cc_default;
   fn_params := nil;
-  fn_vars := nil;
+  fn_vars := ((_result, tint) :: nil);
   fn_body :=
 (Ssequence
   (Ssequence
-    (Sdo (Eassign (Evar _a tint) (Eval (Vint (Int.repr 10)) tint) tint))
+    (Sdo (Eassign (Evar _result tint)
+           (Ecall
+             (Evalof
+               (Evar _add (Tfunction (Tcons tint (Tcons tint Tnil)) tint
+                            cc_default))
+               (Tfunction (Tcons tint (Tcons tint Tnil)) tint cc_default))
+             (Econs (Eval (Vint (Int.repr 3)) tint)
+               (Econs (Eval (Vint (Int.repr 4)) tint) Enil)) tint) tint))
     (Ssequence
-      (Sdo (Eassign (Evar _b tint) (Eval (Vint (Int.repr 15)) tint) tint))
-      (Ssequence
-        (Sdo (Ecall
-               (Evalof (Evar _add (Tfunction Tnil tvoid cc_default))
-                 (Tfunction Tnil tvoid cc_default)) Enil tvoid))
-        (Sreturn (Some (Eval (Vint (Int.repr 0)) tint))))))
+      (Sdo (Ecall
+             (Evalof
+               (Evar _printf (Tfunction (Tcons (tptr tschar) Tnil) tint
+                               {|cc_vararg:=(Some 1); cc_unproto:=false; cc_structret:=false|}))
+               (Tfunction (Tcons (tptr tschar) Tnil) tint
+                 {|cc_vararg:=(Some 1); cc_unproto:=false; cc_structret:=false|}))
+             (Econs
+               (Evalof (Evar ___stringlit_1 (tarray tschar 12))
+                 (tarray tschar 12))
+               (Econs (Evalof (Evar _result tint) tint) Enil)) tint))
+      (Sreturn (Some (Eval (Vint (Int.repr 0)) tint)))))
   (Sreturn (Some (Eval (Vint (Int.repr 0)) tint))))
 |}.
 
@@ -403,29 +397,28 @@ Definition global_definitions : list (ident * globdef fundef type) :=
                      {|cc_vararg:=(Some 1); cc_unproto:=false; cc_structret:=false|}))
      (Tcons (tptr tschar) Tnil) tint
      {|cc_vararg:=(Some 1); cc_unproto:=false; cc_structret:=false|})) ::
- (_a, Gvar v_a) :: (_b, Gvar v_b) :: (_add, Gfun(Internal f_add)) ::
- (_main, Gfun(Internal f_main)) :: nil).
+ (_add, Gfun(Internal f_add)) :: (_main, Gfun(Internal f_main)) :: nil).
 
 Definition public_idents : list ident :=
-(_main :: _add :: _b :: _a :: _printf :: ___builtin_debug ::
- ___builtin_fmin :: ___builtin_fmax :: ___builtin_fnmsub ::
- ___builtin_fnmadd :: ___builtin_fmsub :: ___builtin_fmadd ::
- ___builtin_clsll :: ___builtin_clsl :: ___builtin_cls ::
- ___builtin_expect :: ___builtin_unreachable :: ___builtin_va_end ::
- ___builtin_va_copy :: ___builtin_va_arg :: ___builtin_va_start ::
- ___builtin_membar :: ___builtin_annot_intval :: ___builtin_annot ::
- ___builtin_sel :: ___builtin_memcpy_aligned :: ___builtin_sqrt ::
- ___builtin_fsqrt :: ___builtin_fabsf :: ___builtin_fabs ::
- ___builtin_ctzll :: ___builtin_ctzl :: ___builtin_ctz :: ___builtin_clzll ::
- ___builtin_clzl :: ___builtin_clz :: ___builtin_bswap16 ::
- ___builtin_bswap32 :: ___builtin_bswap :: ___builtin_bswap64 ::
- ___compcert_i64_umulh :: ___compcert_i64_smulh :: ___compcert_i64_sar ::
- ___compcert_i64_shr :: ___compcert_i64_shl :: ___compcert_i64_umod ::
- ___compcert_i64_smod :: ___compcert_i64_udiv :: ___compcert_i64_sdiv ::
- ___compcert_i64_utof :: ___compcert_i64_stof :: ___compcert_i64_utod ::
- ___compcert_i64_stod :: ___compcert_i64_dtou :: ___compcert_i64_dtos ::
- ___compcert_va_composite :: ___compcert_va_float64 ::
- ___compcert_va_int64 :: ___compcert_va_int32 :: nil).
+(_main :: _add :: _printf :: ___builtin_debug :: ___builtin_fmin ::
+ ___builtin_fmax :: ___builtin_fnmsub :: ___builtin_fnmadd ::
+ ___builtin_fmsub :: ___builtin_fmadd :: ___builtin_clsll ::
+ ___builtin_clsl :: ___builtin_cls :: ___builtin_expect ::
+ ___builtin_unreachable :: ___builtin_va_end :: ___builtin_va_copy ::
+ ___builtin_va_arg :: ___builtin_va_start :: ___builtin_membar ::
+ ___builtin_annot_intval :: ___builtin_annot :: ___builtin_sel ::
+ ___builtin_memcpy_aligned :: ___builtin_sqrt :: ___builtin_fsqrt ::
+ ___builtin_fabsf :: ___builtin_fabs :: ___builtin_ctzll ::
+ ___builtin_ctzl :: ___builtin_ctz :: ___builtin_clzll :: ___builtin_clzl ::
+ ___builtin_clz :: ___builtin_bswap16 :: ___builtin_bswap32 ::
+ ___builtin_bswap :: ___builtin_bswap64 :: ___compcert_i64_umulh ::
+ ___compcert_i64_smulh :: ___compcert_i64_sar :: ___compcert_i64_shr ::
+ ___compcert_i64_shl :: ___compcert_i64_umod :: ___compcert_i64_smod ::
+ ___compcert_i64_udiv :: ___compcert_i64_sdiv :: ___compcert_i64_utof ::
+ ___compcert_i64_stof :: ___compcert_i64_utod :: ___compcert_i64_stod ::
+ ___compcert_i64_dtou :: ___compcert_i64_dtos :: ___compcert_va_composite ::
+ ___compcert_va_float64 :: ___compcert_va_int64 :: ___compcert_va_int32 ::
+ nil).
 
 Definition prog : Csyntax.program := 
   mkprogram composites global_definitions public_idents _main Logic.I.
