compiler_test/beepl_test/BeePL_add_ptr.v
@@ -1,0 +1,102 @@
+Require Import Integers AST Ctypes BeePL BeeTypes BeePL_values BeePL_typechecker BeePL_notations. 
+From Coq Require Import String ZArith.
+From compcert Require Import Csyntaxdefs.
+Import Csyntaxdefs.CsyntaxNotations.
+Local Open Scope list_scope.
+Local Open Scope string_scope.
+Local Open Scope csyntax_scope.
+
+(* 
+  int add (int x, int y) 
+      return x + y; *)
+
+(* int main()
+ *   int (star_fp)(int, int) = add;
+ *    int r = fp(2,3);
+ *    return r; *)
+
+
+(* CompCert's memory model does not allow assigning a function address to a function pointer variable in this way:
+   fails at runtime: zsh: bus error  ./a.out *)
+
+Definition dattr := {| attr_volatile := false; attr_alignas := None |}.
+Definition _a : ident := $"a".
+Definition _b : ident := $"b".
+Definition _c : ident := $"c".
+Definition _x : ident := $"x".
+Definition _y : ident := $"y".
+Definition _r : ident := $"r".
+Definition _fp : ident := $"fp".
+Definition _h : ident := $"h". (* supposed to represent heap for Reftype *)
+Definition _add : ident := $"add".
+Definition _main : ident := $"main".
+
+Definition  ident_to_string : list (ident * string) := ((_a, "a") :: 
+                                                        (_b, "b") :: 
+                                                        (_c, "c") ::
+                                                        (_x, "x") :: 
+                                                        (_y, "y") :: 
+                                                        (_r, "r") ::
+                                                        (_fp, "fp") ::
+                                                        (_add, "add") ::
+                                                        (_main, "main") :: nil).
+
+
+Definition f_add : BeePL.function := {| 
+                                   fn_return := tint32u;
+                                   fn_effect := nil;
+                                   fn_callconv := cc_default;
+                                   fn_args := ((_x, tint32u) :: 
+                                               (_y, tint32u) :: nil);
+                                   fn_vars := ((_r, tint32u) :: nil);
+                                   fn_body := Bind 
+                                                (_r) tint32u
+                                                (Prim (Bop Cop.Oadd) 
+                                                      (Var _x tint32u :: 
+                                                       Var _y tint32u :: nil) tint32u)
+                                                (Var _r tint32u) tint32u |}.
+
+Definition f_main : BeePL.function := {| 
+                                   fn_return := tint32u;
+                                   fn_effect := nil;
+                                   fn_callconv := cc_default;
+                                   fn_args := nil;
+                                   fn_vars := ((_a, tint32u) :: 
+                                               (_b, tint32u) ::
+                                               (_fp, (tpfun (tint32u :: tint32u :: nil) nil tint32u)) ::
+                                               (_r, tint32u) :: nil);
+                                   fn_body := 
+                                              Bind 
+                                                   (_a) tint32u
+                                                   (cint (Int.repr 1) tint32u)
+                                                   (Bind (_fp) (tpfun (tint32u :: tint32u :: nil) nil tint32u)
+                                                      (Var _add (tpfun (tint32u :: tint32u :: nil) nil tint32u))
+                                                      (Bind _r tint32u 
+                                                         (App (Var _fp (tpfun (tint32u :: tint32u :: nil) nil tint32u))
+                                                            (Var _a tint32u :: 
+                                                            Var _a tint32u :: nil) tint32u)
+                                                         (Var _r tint32u) tint32u) tunit) tint32u |}.
+
+Definition global_definitions : list (ident * AST.globdef BeePL.fundef type) 
+   := (_add, AST.Gfun(BeePL.Internal (f_add))) ::
+      (_main, AST.Gfun(BeePL.Internal (f_main))) :: nil.
+
+Definition public_idents : list ident := (_main :: _add :: nil).
+
+Definition bcomposites : list bcomposite_definition := nil.
+
+Lemma bcomposite_correct :
+  wf_bcomposites bcomposites.
+Proof.
+  unfold wf_bcomposites.
+  unfold build_bcomposite_env; simpl; reflexivity.
+Qed.
+
+(*Definition example1 : BeePL.program := @mkbprogram bcomposites 
+                                                   global_definitions 
+                                                   public_idents 
+                                                   _main 
+                                                   bcomposite_correct
+                                                   ident_to_string.
+
+Compute (type_check_program example1).*) (* Type checks *)
